Examples.v: progress
Better presentation of cost refining.

The refined expression (before simplification) now only appears in one
place. The subgoal corresponding to the cleanup of the cost function is readable
and doesn't mention explicitly the raw cost function.

The context isn't polluted either, it only contains a definition for the cost
function being elaborated, in the subgoals corresponding to the proof of the
program. The subgoals for "cost function is positive" and "cost function is
dominated by ..." only see the simplified cost function.

examples/proofs/Examples.v
@@ -920,17 +920,41 @@ Ltac hsimpl_setup process_credits ::=
 
 (* todo: notation for to_nat' in order to hide the proof term *)
 
-Ltac cleanup_cost tt :=
+Definition cleanup_cost A (cost cost_clean : A -> Z) :=
+  forall x, cost x = cost_clean x.
+
+Ltac cleanup_cost_core :=
+  repeat rewrite Nat2Z.inj_add;
+  repeat rewrite Z2Nat_id';
+  simpl;
+  ring_simplify.
+
+Ltac cleanup_cost :=
   match goal with
-    |- ?lhs = _ =>
-    let hide_cost := fresh in
-    set (hide_cost := lhs);
-    repeat rewrite Nat2Z.inj_add;
-    repeat rewrite Z2Nat_id';
-    simpl;
-    ring_simplify;
-    subst hide_cost
+    |- cleanup_cost ?cost ?cost_clean =>
+    let cost_clean_ := fresh "cost_clean" in
+    set (cost_clean_ := cost_clean);
+    intro; subst cost; hnf; cleanup_cost_core;
+    subst cost_clean_; reflexivity
   end.
+
+Lemma spec_exists_cost :
+  forall A (cost cost_clean : A -> Z) (P Q R : (A -> Z) -> Prop),
+    P cost ->
+    cleanup_cost cost cost_clean ->
+    Q cost_clean ->
+    R cost_clean ->
+    (exists cost, P cost /\ Q cost /\ R cost).
+Proof.
+  intros ? cost_ cost_clean.
+  introv HP E HQ HR.
+  forwards E': func_ext_dep E.
+  exists cost_.
+  splits.
+  assumption.
+  rewrite E'. assumption.
+  rewrite E'. assumption.
+Qed.
 
 Lemma let1_spec :
   exists (cost : Z -> Z),
@@ -943,9 +967,15 @@ Lemma let1_spec :
   dominated Z_filterType cost (fun (n:Z) => n).
 Proof.
   destruct loop1_spec_2 as (loop1_cost & L & LP & LD).
-  eexists. splits. intros n N.
 
-  eapply spec_cost_is_constant.
+  evar (cost : Z -> Z). evar (cost_clean : Z -> Z).
+  apply (@spec_exists_cost Z cost cost_clean); subst cost_clean;
+    [ | | subst cost | subst cost ].
+
+  intros n N.
+
+  (* en fait facultatif *)
+  eapply spec_cost_is_constant; [| reflexivity].
 
   xcf.
   xpay.
@@ -958,7 +988,7 @@ Proof.
 
   subst m. hsimpl. apply LP.
 
-  cleanup_cost tt. reflexivity.
+  cleanup_cost.
 
   { intros x. simpl. auto with zarith. }
   { apply dominated_sum_distr.
